Upd

VRF/VRF.fst
@@ -8,10 +8,15 @@ open Hacl.UInt8
 open Hacl.UInt32
 open FStar.UInt32
 
-open Hacl.Impl.Ed25519.ExtPoint
+open Hacl.Bignum25519
+open Hacl.Impl.Ed25519.PointAdd
 
+open Hacl.Impl.Ed25519.ExtPoint
+open Hacl.Impl.Ed25519.PointCompress
 
 type bytes = buffer FStar.UInt8.t
+type hbytes = buffer Hacl.UInt8.t
+
 private let uint32_t  = FStar.UInt32.t
 private let uint64_t = FStar.UInt64.t
 
@@ -28,181 +33,228 @@ let n = 32ul
 
 
 assume val hash: hash: bytes {length hash = v size_hash} ->
-    input: bytes {length input < max_input_len_8 /\ disjoint hash input} -> 
-    len : uint32_t {v len = length input} -> 
-    Stack unit 
-        (requires 
-            (fun h0 -> live h0 hash /\ live h0 input))
-        (ensures    
-            (fun h0 _ h1 -> live h0 input /\ live h0 hash /\ live h1 hash /\ modifies_1 hash h0 h1))
+	input: bytes {length input < max_input_len_8 /\ disjoint hash input} -> 
+	len : uint32_t {v len = length input} -> 
+	Stack unit 
+		(requires 
+			(fun h0 -> live h0 hash /\ live h0 input))
+		(ensures	
+			(fun h0 _ h1 -> live h0 input /\ live h0 hash /\ live h1 hash /\ modifies_1 hash h0 h1))
 
-assume val scalarAddition: out: point ->
-    p: point -> 
-    q: point -> 
-    Stack unit 
-        (requires
-            (fun h0 -> live h0 out /\ live h0 p /\ live h0 q)
-        )
-        (ensures 
-            (fun h0  _ h1 -> live h0 out /\ live h0 p /\ live h0 q /\ modifies_1 out h0 h1)
-        )
+val scalarAddition:
+  out:point ->
+  p:point{disjoint p out} ->
+  q:point{disjoint q out} ->
+  Stack unit
+    (requires (fun h -> live h out /\ live h p /\ live h q  /\
+      (
+        let x1 = as_seq h (getx p) in
+        let y1 = as_seq h (gety p) in
+        let z1 = as_seq h (getz p) in
+        let t1 = as_seq h (gett p) in
+
+        let x2 = as_seq h (getx q) in
+        let y2 = as_seq h (gety q) in
+        let z2 = as_seq h (getz q) in
+        let t2 = as_seq h (gett q) in
+        red_513 x1 /\ red_513 y1 /\ red_513 z1 /\ red_513 t1 /\
+        red_513 x2 /\ red_513 y2 /\ red_513 z2 /\ red_513 t2)
+      ))
+    (ensures (fun h0 _ h1 -> live h1 out /\ live h0 p /\ live h0 q /\ modifies_1 out h0 h1 /\
+      (
+        let x1 = as_seq h0 (getx p) in
+        let y1 = as_seq h0 (gety p) in
+        let z1 = as_seq h0 (getz p) in
+        let t1 = as_seq h0 (gett p) in
+        let x2 = as_seq h0 (getx q) in
+        let y2 = as_seq h0 (gety q) in
+        let z2 = as_seq h0 (getz q) in
+        let t2 = as_seq h0 (gett q) in
+        let x3 = as_seq h1 (getx out) in
+        let y3 = as_seq h1 (gety out) in
+        let z3 = as_seq h1 (getz out) in
+        let t3 = as_seq h1 (gett out) in
+        (seval x3, seval y3, seval z3, seval t3) ==
+          Spec.Ed25519.point_add (seval x1, seval y1, seval z1, seval t1)
+                                 (seval x2, seval y2, seval z2, seval t2)
+        /\ red_513 x3 /\ red_513 y3 /\ red_513 z3 /\ red_513 t3)
+  ))
+
+let scalarAddition out p q = 
+	point_add out p q
 
 assume val scalarMultiplication : out: point -> p: point ->  k:buffer Hacl.UInt8.t{length k = 32 } -> 
-    Stack unit
-        (requires
-            (fun h0 -> live h0 p /\ live h0 k /\ live h0 out)
-        )
-        (ensures
-            (fun h0 _ h1 -> live h1 p /\ live h1 k /\ live h0 out /\ modifies_1 k h0 h1)    
-        )
+	Stack unit
+		(requires
+			(fun h0 -> live h0 p /\ live h0 k /\ live h0 out)
+		)
+		(ensures
+			(fun h0 _ h1 -> live h1 p /\ live h1 k /\ live h0 out /\ modifies_1 k h0 h1)	
+		)
 
 assume val isPointOnCurve: p: point -> Stack bool
-    (requires (fun h0 -> live h0 p))    
-    (ensures (fun h0 _ h1 -> live h1 p))    
+	(requires (fun h0 -> live h0 p))	
+	(ensures (fun h0 _ h1 -> live h1 p))	
 
-assume val _ECP2OS: out: bytes -> p: point -> Stack unit 
-    (ensures(fun h0 -> live h0 out /\ live h0 p))
-    (ensures(fun h0 _ h1 -> live h1 p /\ live h1 out /\ modifies_1 out h0 h1))
+val _ECP2OS: out: hbytes{length out = 32} -> p: point -> Stack unit 
+	(requires
+		(fun h0 -> live h0 out /\ live h0 p  /\
+			red_513 (as_seq h0 (Hacl.Impl.Ed25519.ExtPoint.getx p)) /\
+			red_513 (as_seq h0 (Hacl.Impl.Ed25519.ExtPoint.gety p)) /\
+			red_513 (as_seq h0 (Hacl.Impl.Ed25519.ExtPoint.getz p)) /\
+			red_513 (as_seq h0 (Hacl.Impl.Ed25519.ExtPoint.gett p))
+		)
+	)
+	(ensures
+		(fun h0 _ h1 -> 
+			live h0 out /\ live h1 out /\ live h1 p /\  modifies_1 out h0 h1 
+			(*/\ h1.[out] == Spec.Ed25519.point_compress(Hacl.Impl.Ed25519.ExtPoint.as_point h0 p)*)
+		)
+	)
 
-assume val random: random: bytes {length random = 32} ->     
-    Stack unit 
-        (requires 
-            (fun h0 -> live h0 random)
-        )
-        (ensures 
-            (fun h0 _ h1 -> live h0 random /\ modifies_1 random h0 h1)
-        )
+let _ECP2OS out p = point_compress out p
+
+
+
+assume val random: random: bytes {length random = 32} -> 	
+	Stack unit 
+		(requires 
+			(fun h0 -> live h0 random)
+		)
+		(ensures 
+			(fun h0 _ h1 -> live h0 random /\ modifies_1 random h0 h1)
+		)
 
 assume val _ECVRF_hash_to_curve:
-    output: point -> 
-    input: bytes {length input < max_input_len_8 - 36} ->
-    len_input : uint32_t {v len_input = length input} -> 
-    public_key: point -> 
-    Stack bool 
-        (requires
-            (fun h0 -> live h0 output /\ live h0 input /\ live h0 public_key)
-        )
-        (ensures
-            (fun h0 _ h1 -> live h1 output /\ live h1 input /\ live h1 public_key /\ modifies_1 output h0 h1)
-        )
+	output: point -> 
+	input: bytes {length input < max_input_len_8 - 36} ->
+	len_input : uint32_t {v len_input = length input} -> 
+	public_key: point -> 
+	Stack bool 
+		(requires
+			(fun h0 -> live h0 output /\ live h0 input /\ live h0 public_key)
+		)
+		(ensures
+			(fun h0 _ h1 -> live h1 output /\ live h1 input /\ live h1 public_key /\ modifies_1 output h0 h1)
+		)
 
 assume val _ECVRF_hash_points: out: bytes -> 
-    p1: point -> 
-    p2:point -> 
-    p3: point ->
-    p4: point -> 
-    p5: point -> 
-    p6: point -> 
-    Stack unit 
-        (requires
-            (fun h0 ->live h0 out /\ live h0 p1 /\  live h0 p2 /\  live h0 p3 /\  live h0 p4 /\  live h0 p5 /\  live h0 p6 )
-        )
+	p1: point -> 
+	p2:point -> 
+	p3: point ->
+	p4: point -> 
+	p5: point -> 
+	p6: point -> 
+	Stack unit 
+		(requires
+			(fun h0 ->live h0 out /\ live h0 p1 /\  live h0 p2 /\  live h0 p3 /\  live h0 p4 /\  live h0 p5 /\  live h0 p6 )
+		)
 
-        (ensures
-            (fun h0 _ h1 -> live h0 out /\ live h0 p1 /\  live h0 p2 /\  
-            live h0 p3 /\  live h0 p4 /\  live h0 p5 /\  live h0 p6 /\ modifies_1 out h0 h1 )
-        )
+		(ensures
+			(fun h0 _ h1 -> live h0 out /\ live h0 p1 /\  live h0 p2 /\  
+			live h0 p3 /\  live h0 p4 /\  live h0 p5 /\  live h0 p6 /\ modifies_1 out h0 h1 )
+		)
 
 assume val pointCreate: unit -> Stack (p:point)
-        (requires 
-            (fun h0 -> true)
-        )
-        (ensures
-            (fun h0 r h1 -> true)
-        )
+		(requires 
+			(fun h0 -> true)
+		)
+		(ensures
+			(fun h0 r h1 -> true)
+		)
 (*))
 assume val testFunc : p: point -> Stack unit 
-    (requires
-        (fun h0 -> live h0 p)
-    )
-    (ensures
-        (fun h0 _ h1 -> live h1 p)
-    )
+	(requires
+		(fun h0 -> live h0 p)
+	)
+	(ensures
+		(fun h0 _ h1 -> live h1 p)
+	)
 
 val a: unit -> Stack unit
-    (requires (fun h0 -> true))
-    (ensures (fun h0 _ h1 -> true))
+	(requires (fun h0 -> true))
+	(ensures (fun h0 _ h1 -> true))
 
 let a () = 
-    let point = pointCreate () in 
-    testFunc point; ()
+	let point = pointCreate () in 
+	testFunc point; ()
 *)
 
 
 
 assume val bytesMultiplication: out: bytes -> m1: bytes -> m2 : uint64_t -> mod: uint64_t -> Stack unit 
-    (requires (fun h0 -> live h0 out /\ live h0 m1))
-    (ensures (fun h0 _ h1 -> live h1 m1 /\ modifies_1 out h0 h1))
+	(requires (fun h0 -> live h0 out /\ live h0 m1))
+	(ensures (fun h0 _ h1 -> live h1 m1 /\ modifies_1 out h0 h1))
 
 assume val bytesInverse: out: bytes -> m: bytes -> Stack unit
-    (requires(fun h0 -> live h0 out /\ live h0 m))
-    (ensures (fun h0 _ h1 -> live h1 m /\ modifies_1 out h0 h1))    
+	(requires(fun h0 -> live h0 out /\ live h0 m))
+	(ensures (fun h0 _ h1 -> live h1 m /\ modifies_1 out h0 h1))	
 
 assume val bytesAddition: out: bytes -> m1: bytes -> m2: bytes -> Stack unit
-    (requires (fun h0 -> live h0 out /\ live h0 m1 /\ live h0 m2))
-    (ensures (fun h0 _ h1 -> live h1 out /\ modifies_1 out h0 h1 /\ live h1 m1 /\ live h1 m2))
+	(requires (fun h0 -> live h0 out /\ live h0 m1 /\ live h0 m2))
+	(ensures (fun h0 _ h1 -> live h1 out /\ modifies_1 out h0 h1 /\ live h1 m1 /\ live h1 m2))
 
 assume val bytesConcat: out: bytes -> m1: bytes -> m2: bytes -> Stack unit
-    (requires (fun h0 -> live h0 out /\ live h0 m1 /\ live h0 m2))
-    (ensures (fun h0 _ h1 -> live h1 out /\ live h1 m1 /\ live h1 m2 /\ modifies_1 out h0 h1))
+	(requires (fun h0 -> live h0 out /\ live h0 m1 /\ live h0 m2))
+	(ensures (fun h0 _ h1 -> live h1 out /\ live h1 m1 /\ live h1 m2 /\ modifies_1 out h0 h1))
 
 assume val bytesSplit: out: bytes -> m: bytes ->  p1: int -> p2: int -> Stack unit
-    (requires (fun h0 -> live h0 out /\ live h0 m))
-    (ensures (fun h0 _ h1 -> live h1 out /\ live h1 m /\ modifies_1 out h0 h1 ))
+	(requires (fun h0 -> live h0 out /\ live h0 m))
+	(ensures (fun h0 _ h1 -> live h1 out /\ live h1 m /\ modifies_1 out h0 h1 ))
 
 val _ECVRF_prove: 
-    proof: bytes {length proof = v (n *^ 4ul) } ->
-    input: bytes {length input < max_input_len_8 - 36  } ->
-    len_input : uint32_t {v len_input = length input} -> 
-    public_key: point -> 
-    private_key: buffer Hacl.UInt8.t {length private_key = 32} -> 
-    generator: point -> 
-    field: uint64_t -> 
-    Stack bool 
-        (requires 
-            (fun h0 -> live h0 input /\ live h0 public_key /\ live h0 private_key /\ live h0 generator /\ live h0 proof )
-        )
-        (ensures
-            (fun h0 _ h1 -> live h0 input /\ live h0 public_key /\ 
-            live h0 private_key /\ live h0 generator /\ live h0 proof /\ modifies_1 proof h0 h1)
-        )
+	proof: bytes {length proof = v (n *^ 4ul) } ->
+	input: bytes {length input < max_input_len_8 - 36  } ->
+	len_input : uint32_t {v len_input = length input} -> 
+	public_key: point -> 
+	private_key: buffer Hacl.UInt8.t {length private_key = 32} -> 
+	generator: point -> 
+	field: uint64_t -> 
+	Stack bool 
+		(requires 
+			(fun h0 -> live h0 input /\ live h0 public_key /\ live h0 private_key /\ live h0 generator /\ live h0 proof )
+		)
+		(ensures
+			(fun h0 _ h1 -> live h0 input /\ live h0 public_key /\ 
+			live h0 private_key /\ live h0 generator /\ live h0 proof /\ modifies_1 proof h0 h1)
+		)
 
 let _ECVRF_prove proof input len_input public_key private_key generator field  = 
-    let h = pointCreate() in 
-    let hashResult = _ECVRF_hash_to_curve h input len_input public_key in 
-        if hashResult = false then false else 
-        let gamma = pointCreate () in 
-    scalarMultiplication gamma h private_key; 
-        let k = create 0uy 32ul in 
-        let gk = pointCreate() in 
-        let hk = pointCreate() in 
-    random k; 
-    scalarMultiplication gk generator k;
-    scalarMultiplication hk h k;
-        let c = create 0uy 32ul in
-    _ECVRF_hash_points c generator h public_key gamma gk hk; 
-        let cqmod = create 0uy 32ul in 
-    bytesMultiplication cqmod c field field; (* smaller than field*)
-    bytesInverse cqmod cqmod;
-        let s = create 0uy 32ul in 
-    bytesAddition s k cqmod;
-        let fstsnd = create 0uy 64ul in 
-        let fst = create 0uy 32ul in 
-    _ECP2OS fst gamma;
-    bytesConcat fstsnd fst c;
-    bytesConcat proof fstsnd s; true
+	let h = pointCreate() in 
+	let hashResult = _ECVRF_hash_to_curve h input len_input public_key in 
+		if hashResult = false then false else 
+		let gamma = pointCreate () in 
+	scalarMultiplication gamma h private_key; 
+		let k = create 0uy 32ul in 
+		let gk = pointCreate() in 
+		let hk = pointCreate() in 
+	random k; 
+	scalarMultiplication gk generator k;
+	scalarMultiplication hk h k;
+		let c = create 0uy 32ul in
+	_ECVRF_hash_points c generator h public_key gamma gk hk; 
+		let cqmod = create 0uy 32ul in 
+	bytesMultiplication cqmod c field field; (* smaller than field*)
+	bytesInverse cqmod cqmod;
+		let s = create 0uy 32ul in 
+	bytesAddition s k cqmod;
+		let fstsnd = create 0uy 64ul in 
+		let fst = create 0uy 32ul in 
+	_ECP2OS fst gamma;
+	bytesConcat fstsnd fst c;
+	bytesConcat proof fstsnd s; true
 
 val _ECVRF_proof2hash: out: bytes -> proof: bytes -> Stack unit
 (requires (fun h0 -> live h0 out /\ live h0 proof))
 (ensures (fun h0 _ h1 -> live h1 out /\ live h1 proof))
 
 let _ECVRF_proof2hash out proof = 
-    bytesSplit out proof 0 1
+	bytesSplit out proof 0 1
 
 assume val _ECVRF_decode_proof: gamma:  point -> c: bytes -> s : bytes -> pi: bytes -> Stack bool
 (requires (fun h0 -> live h0 gamma /\ live h0 c /\ live h0 s /\ live h0 pi))
 (ensures (fun h0 _ h1 -> live h1 gamma /\ live h1 c /\ live h1 s /\ 
-    live h1 pi /\ modifies_1 gamma h0 h1 /\ modifies_1 c h0 h1 /\ modifies_1 s h0 h1 ))
+	live h1 pi /\ modifies_1 gamma h0 h1 /\ modifies_1 c h0 h1 /\ modifies_1 s h0 h1 ))
 
 
 val _ECVRF_verify: generator: point -> public_key : point -> pi: bytes -> input: bytes ->
@@ -211,28 +263,28 @@ len_input : uint32_t {v len_input = length input} ->  Stack bool
 (ensures (fun h0 _ h1 -> live h1 generator /\ live h1 public_key /\ live h1 pi /\ live h1 input))
 
 let _ECVRF_verify generator public_key pi input len_input = 
-        let gamma = pointCreate () in 
-        let c = create 0uy 32ul in  
-        let s = create 0uy 32ul in 
-    let decoded = _ECVRF_decode_proof gamma c s pi in 
-        if not(decoded)  then false 
-        else if not(isPointOnCurve gamma) then false
-        else 
-        let pkc = pointCreate() in 
-        let gs = pointCreate() in 
-    scalarMultiplication pkc public_key c;
-    scalarMultiplication gs generator s;
-        let u = pointCreate () in 
-    scalarAddition u pkc gs; 
-        let h = pointCreate () in 
-    let h_ = _ECVRF_hash_to_curve h input len_input public_key in 
-        if not(h_) then false else 
-        let gammac = pointCreate() in 
-        let hs = pointCreate() in 
-    scalarMultiplication gammac gamma c; 
-    scalarMultiplication hs h s;     
-        let v = pointCreate() in 
-    scalarAddition v gammac hs; 
-        let c_prime = create 0uy 32ul in 
-    _ECVRF_hash_points c_prime generator h public_key gamma u v;
-    (c = c_prime)
+		let gamma = pointCreate () in 
+		let c = create 0uy 32ul in  
+		let s = create 0uy 32ul in 
+	let decoded = _ECVRF_decode_proof gamma c s pi in 
+		if not(decoded)  then false 
+		else if not(isPointOnCurve gamma) then false
+		else 
+		let pkc = pointCreate() in 
+		let gs = pointCreate() in 
+	scalarMultiplication pkc public_key c;
+	scalarMultiplication gs generator s;
+		let u = pointCreate () in 
+	scalarAddition u pkc gs; 
+		let h = pointCreate () in 
+	let h_ = _ECVRF_hash_to_curve h input len_input public_key in 
+		if not(h_) then false else 
+		let gammac = pointCreate() in 
+		let hs = pointCreate() in 
+	scalarMultiplication gammac gamma c; 
+	scalarMultiplication hs h s; 	
+		let v = pointCreate() in 
+	scalarAddition v gammac hs; 
+		let c_prime = create 0uy 32ul in 
+	_ECVRF_hash_points c_prime generator h public_key gamma u v;
+	(c = c_prime)
